\lambda -> SK

scripts/ToSk.hs
@@ -1,0 +1,49 @@
+data LExpr = Lam LExpr
+  | Var Int
+  | App LExpr LExpr
+  | Me
+  | Ke
+  | Se
+
+data SkExpr = S
+  | K
+  | M
+  | Call SkExpr SkExpr
+  | Const String
+  | Placeholder
+
+tosk :: LExpr -> SkExpr
+tosk Me = M
+tosk Se = S
+tosk Ke = K
+tosk (Lam x (Var 1)) = Call (Call (S (M K)) K) K
+tosk (Lam x (App lhs rhs)) = let sklhs = (tosk $ Lam x lhs) in
+  let skrhs = (tosk $ Lam x rhs) in
+  (Call (Call S sklhs) skrhs)
+tosk (Lam x otherwise) = Call K (tosk otherwise)
+tosk (App lhs rhs) = Call (tosk lhs) (tosk rhs)
+tosk (Var bruh) = Call K (Const bruh)
+
+typeof :: SkExpr -> SkExpr
+typeof x = (Call M x)
+
+typify :: SkExpr -> SkExpr
+typify (Call K a) = (Call (Call (Call K (Call M a)) Placeholder) a)
+typify ((Call K a) b) = (Call (Call (Call (Call K (Call M a)) (Call M b)) a) b)
+typify (Call (Call (Call S x) y) z) = (((Call S (Call M x)) (Call M y)) (Call M z))
+
+eval :: SkExpr -> SkExpr
+eval (Call (Call (Call (Call K a) b) x) y) = x
+eval (Call (Call (Call (Call (Call (Call S a) b) c) x) y) z) = eval (Call (Call x z) (Call y z))
+eval x = x
+
+instance Show SkExpr where
+  show M = "M"
+  show S = "S"
+  show K = "K"
+  show (Call lhs rhs) = "(" ++ (show lhs) ++ " " ++ (show rhs) ++ ")"
+  show (Const c) = show c
+
+main :: IO ()
+main =
+  putStrLn $ show $ eval $ tosk (Lam (Lam (App (App (App Ke (App Me (Var 1))) (Var 2)) (Var 1))))
