SkLean/Ast2.lean
@@ -1,11 +1,45 @@
 import Mathlib.Tactic
 
+/-
+# Hierarchied, Reflective SK
+
+I want to make the SK combinators more expressive while maintaining simplicity. I also want to make a proof assistant based on them. In order to formalize properties of the combinators, we required a type system. We have seen thus far the typical typing of \\(K : \alpha \rightarrow \beta \rightarrow \alpha\\). I propose a binderless, expressive type system for the combinators featuring reflection.
+
+## Type Constructors
+
+The \\(K\\) and \\(S\\) combinators double as type constructors in my calculus. I define a mapping from the combinators to arrows:
+
+$$
+K : \alpha \rightarrow \beta \rightarrow \alpha
+$$
+
+For example, to construct the arrow \\(\alpha \rightarrow \alpha\\):
+
+$$
+SKS : \alpha \rightarrow \alpha
+$$
+
+- M is computable. It is not a type.
+-/
+
 inductive Expr where
   | m    : ℕ → Expr
   | k    : ℕ → Expr
   | s    : ℕ → Expr
   | call : Expr → Expr → Expr
 deriving DecidableEq, Repr, BEq
+
+namespace Expr
+
+def sum_universes (e : Expr) : ℕ :=
+  match e with
+    | .m n => n
+    | .k n => n
+    | .s n => n
+    | .call lhs rhs =>
+      lhs.sum_universes + rhs.sum_universes
+
+end Expr
 
 /-
 ## DSL
@@ -17,141 +51,65 @@ declare_syntax_cat skmexpr
 syntax "K" term                : skmexpr
 syntax "S" term                : skmexpr
 syntax "M" term                : skmexpr
-syntax "K" num                 : skmexpr
-syntax "S" num                 : skmexpr
-syntax "M" num                 : skmexpr
 syntax "(" skmexpr skmexpr ")" : skmexpr
 syntax ident                   : skmexpr
 syntax "#" term                : skmexpr
 syntax "(" skmexpr ")"         : skmexpr
 
 syntax " ⟪ " skmexpr " ⟫ "     : term
-
-macro_rules
-  | `(⟪ K $u:term ⟫)                      => `(Expr.k $u)
-  | `(⟪ S $u:term ⟫)                      => `(Expr.s $u)
-  | `(⟪ M $u:term ⟫)                      => `(Expr.m $u)
-  | `(⟪ K $u:num ⟫)                       => `(Expr.k $u)
-  | `(⟪ S $u:num ⟫)                       => `(Expr.s $u)
-  | `(⟪ M $u:num ⟫)                       => `(Expr.m $u)
-  | `(⟪ $e:ident ⟫)                       => `($e)
-  | `(⟪ # $e:term ⟫)                      => `($e)
-  | `(⟪ ($e:skmexpr) ⟫)                   => `(⟪$e⟫)
-  | `(⟪ ($e₁:skmexpr $e₂:skmexpr) ⟫)      => `(Expr.call ⟪ $e₁ ⟫ ⟪ $e₂ ⟫)
-
-syntax "SKM[ " skmexpr " ] "      : term
+syntax "SKM[ " skmexpr " ] "   : term
 
 macro_rules
   | `(SKM[ $e:skmexpr ]) => `(⟪ $e ⟫)
 
-/-
-## Judgment Rules
+macro_rules
+  | `(⟪ K $e:term ⟫)                 => `(Expr.k $e)
+  | `(⟪ S $e:term ⟫)                 => `(Expr.s $e)
+  | `(⟪ M $e:term ⟫)                 => `(Expr.m $e)
+  | `(⟪ $e:ident ⟫)                  => `($e)
+  | `(⟪ # $e:term ⟫)                 => `($e)
+  | `(⟪ ($e:skmexpr) ⟫)              => `(⟪$e⟫)
+  | `(⟪ ($e₁:skmexpr $e₂:skmexpr) ⟫) => `(Expr.call ⟪ $e₁ ⟫ ⟪ $e₂ ⟫)
 
-`K`, `M`, and `S` must be well-typed on their own. We need some expression that can represent the type of `K`. One option is the \\(\rightarrow\\) type constructor from the SLTC or System F. The typing of \\(S\\) and \\(K\\) are fairly obvious. However, the typing of \\(M\\) is not. It's not immediately clear that we need typing judgment rules for `K`, `M`, or `S` alone. There is no way to explicitly assign a type to `K`, `M`, or `S`. They just are. However, there are emergent rules for application. The typical rules for application in the SK combinator calculus are as follows:
-
-$$
-K : \alpha \rightarrow \beta \rightarrow \alpha \\\\
-S : (\alpha \rightarrow \beta \rightarrow \gamma) \rightarrow (\alpha \rightarrow \beta) \rightarrow \alpha \rightarrow \gamma \\\\
-M : hmm
-$$
-
-Typing rules quickly beome complicated. We would prefer to avoid binders in our type discipline. We can create an "emergent" typing based on function application.
-
-$$
-\frac{
-  \Gamma \vdash e_{1} : T
-}{
-  \Gamma \vdash K\ e_{1}\ e_{2} : T
-}
-$$
-$$
-\frac{
-  \Gamma \vdash f_{1}\ \text{arg}\ (f_{2}\ \text{arg}) : T)
-}{
-  \Gamma \vdash S\ f_{1}\ f_{2}\ \text{arg} : T
-}
-$$
-
-But what is the type of \\(K\\)? It's not really obvious. Clearly, we need some way to represent the type of \\(K\\) that avoids binders. Recall that:
-
-$$
-Kxy = x
-$$
-
-The type of \\(K\\) is typically \\(\alpha \rightarrow \beta \rightarrow \alpha\\). Its type is of the form of the \\(K\\) combinator. We can thus define a typing as such:
-
-$$
-K : K
-$$
-
-This typing is coherent under an evaluation rule for the \\(M\\) combinator:
-
-$$
-M\ (x : t)\ \text{arg} = \text{arg}\ x\ (\text{arg}\ t) \\\\
-M\ \mathbb{N}\ K = K\ \mathbb{N}\ (K\ \text{Type}) = \mathbb{N} \\\\
-M\ K\ K = K\ K\ (K\ K) = K
-$$
--/
-
-namespace Expr
-
-def sum_universes (e : Expr) : ℕ :=
-  match e with
-    | SKM[(K n)] => n
-    | SKM[(S n)] => n
-    | SKM[(M n)] => n
-    | SKM[(lhs rhs)] => sum_universes lhs + sum_universes rhs
-
-end Expr
-
-@[simp]
-abbrev trivial_typing (e : Expr) : Expr := SKM[((M e.sum_universes.succ) e)]
+def implies (α β : Expr) : Expr :=
+  let ty_β := SKM[((M β.sum_universes.succ) β)]
+  SKM[((((K ty_β.sum_universes.succ) (ty_β)) α) β)]
 
 inductive is_eval_once : Expr → Expr → Prop
-  | k x y n      : is_eval_once SKM[(((K n) x) y)] x
-  | s x y z n    : is_eval_once SKM[((((S n) x) y) z)] SKM[((x z) (y z))]
-  | m_k          : is_eval_once SKM[((M n.succ) (K n))] SKM[(K n.succ)]
-  | m_s          : is_eval_once SKM[((M n.succ) (S n))] SKM[(S n.succ)]
-  | m_m          : is_eval_once SKM[((M n.succ) (M n))] SKM[(M n.succ)]
-  | m_call       : is_eval_once SKM[((M SKM[(lhs rhs)].sum_universes.succ) (lhs rhs))]
+  | k x y        : is_eval_once SKM[(((((K n) _α) _β) x) y)] x
+  | s x y z      : is_eval_once SKM[(((((((S n) _α) _β) _γ) x) y) z)] SKM[((x z) (y z))]
+  | m_k          : is_eval_once SKM[((M n.succ) (K n))] SKM[K n.succ]
+  | m_s          : is_eval_once SKM[((M n.succ) (S n))] SKM[S n.succ]
+  | m_m          : is_eval_once SKM[((M n.succ) (M n))] SKM[M n.succ]
+  | m_call       : is_eval_once SKM[((M n) (lhs rhs))]
     SKM[(((M lhs.sum_universes.succ) lhs) ((M rhs.sum_universes.succ) rhs))]
-  | left         : is_eval_once lhs lhs' → is_eval_once SKM[(lhs rhs)] SKM[(lhs' rhs)]
 
-inductive beta_eq : SkExpr → SkExpr → Prop
-  | rfl                       : beta_eq e e
-  | eval                      : is_eval_once e₁ e₂ → beta_eq e₁ e₂
-  | left                      : beta_eq lhs lhs'   → beta_eq SKM[(lhs rhs)] SKM[(lhs' rhs)]
-  | right                     : beta_eq rhs rhs'   → beta_eq SKM[(lhs rhs)] SKM[(lhs rhs')]
-  | trans                     : beta_eq e₁ e₂      → beta_eq e₂ e₃ → beta_eq e₁ e₃
-  | symm                      : beta_eq e₁ e₂      → beta_eq e₂ e₁
+inductive step_eval : Expr → Expr → Prop
+  | once  : is_eval_once e e' → step_eval e e'
+  | left  : step_eval lhs lhs'
+    → step_eval SKM[(lhs rhs)] SKM[(lhs' rhs)]
+  | right : step_eval rhs rhs'
+    → step_eval SKM[(lhs rhs)] SKM[(lhs rhs')]
+
+inductive beta_eq : Expr → Expr → Prop
+  | rfl   : beta_eq e e
+  | eval  : step_eval e₁ e₂  → beta_eq e₁ e₂
+  | left  : beta_eq lhs lhs' → beta_eq SKM[(lhs rhs)] SKM[(lhs' rhs)]
+  | right : beta_eq rhs rhs' → beta_eq SKM[(lhs rhs)] SKM[(lhs rhs')]
+  | trans : beta_eq e₁ e₂    → beta_eq e₂ e₃ → beta_eq e₁ e₃
+  | symm  : beta_eq e₁ e₂    → beta_eq e₂ e₁
 
 inductive valid_judgment : Expr → Expr → Prop
-  | k n                       : valid_judgment SKM[K n] (trivial_typing SKM[(K n)])
-  | s n                       : valid_judgment SKM[S n] (trivial_typing SKM[(S n)])
-  | m n                       : valid_judgment SKM[M n] (trivial_typing SKM[(M n)])
-  | call_k₁                   : valid_judgment x t_x
-    → valid_judgment SKM[((K n) x)] (trivial_typing SKM[((K n) x)])
-  | call_s₁                   : valid_judgment x t_x
-    → valid_judgment SKM[((S n) x)] (trivial_typing SKM[((S n) x)])
-  | call_s₂                   : valid_judgment x t_x
-    → valid_judgment y t_y
-    → valid_judgment SKM[(((S n) x) y)] (trivial_typing SKM[(((S n) x) y)])
-  | call_k                    : valid_judgment x t_x
-    → valid_judgment y t_y
-    → valid_judgment SKM[(((K n) x) y)] (trivial_typing SKM[(((K n) x) y)])
-  | call_s                    : valid_judgment SKM[((x z) (y z))] t_call
-    → valid_judgment x t_x
-    → valid_judgment y t_y
-    → valid_judgment z t_z
-    → SKM[((x z) (y z))].sum_universes < SKM[(((((S n) x) y) z))].sum_universes
-    → valid_judgment SKM[((((S n) x) y) z)] (trivial_typing SKM[((((S n) x) y) z)])
-  | call_m                    : valid_judgment e t
-    → valid_judgment SKM[((M n) e)] (trivial_typing SKM[((M n) e)])
-  | call                      : valid_judgment lhs t_lhs
-    → valid_judgment rhs t_rhs
-    → is_eval_once SKM[(lhs rhs)] e'
-    → SKM[(lhs rhs)].sum_universes < e'.sum_universes
-    → valid_judgment SKM[(lhs rhs)] (trivial_typing SKM[(lhs rhs)])
+  | k                         : valid_judgment SKM[K n] SKM[K n.succ]
+  | s                         : valid_judgment SKM[S n] SKM[S n.succ]
+  | m                         : valid_judgment SKM[M n] SKM[M n.succ]
+  | call_k                    : valid_judgment x α
+    → valid_judgment y β
+    → valid_judgment SKM[(((((K n) α) β) x) y)] α
+  | call_s                    : valid_judgment x SKM[(((K n) α) β)]
+    → valid_judgment y SKM[((((K n) β) α) x_in_val)]
+    → valid_judgment z α
+    → valid_judgment SKM[(((((((S n) α) β) γ) x) y) z)] γ
 
 inductive is_normal_n : ℕ → Expr → Expr → Prop
   | stuck : (¬(∃ e', is_eval_once e e'))                 → is_normal_n 0 e e
@@ -159,22 +117,65 @@ inductive is_normal_n : ℕ → Expr → Expr → Prop
 
 namespace is_normal_n
 
-lemma m_stuck : is_normal_n 0 SKM[M n] SKM[M n] := by
+lemma m_stuck : is_normal_n 0 SKM[M] SKM[M] := by
   apply is_normal_n.stuck
   intro h
   obtain ⟨e', h_eval⟩ := h
   cases h_eval
 
-lemma k_stuck : is_normal_n 0 SKM[K n] SKM[K n] := by
+lemma k_stuck : is_normal_n 0 SKM[K] SKM[K] := by
   apply is_normal_n.stuck
   intro h
   obtain ⟨e', h_eval⟩ := h
   cases h_eval
 
-lemma s_stuck : is_normal_n 0 SKM[S n] SKM[S n] := by
+lemma s_stuck : is_normal_n 0 SKM[S] SKM[S] := by
   apply is_normal_n.stuck
   intro h
   obtain ⟨e', h_eval⟩ := h
   cases h_eval
 
 end is_normal_n
+
+namespace beta_eq
+
+@[simp]
+lemma m_distributes : beta_eq SKM[(M (lhs rhs))] SKM[((M lhs) (M rhs))] := by
+  apply beta_eq.eval
+  apply step_eval.once
+  apply is_eval_once.m_call
+
+lemma funext : beta_eq e₁ e' → beta_eq e₂ e' → beta_eq e₁ e₂ := by
+  intro h_beq₁ h_beq₂
+  induction h_beq₁
+  exact beta_eq.symm h_beq₂
+  case eval h =>
+    apply beta_eq.symm
+    apply beta_eq.trans
+    exact h_beq₂
+    exact beta_eq.symm (beta_eq.eval h)
+  case left =>
+    apply beta_eq.trans
+    apply beta_eq.left
+    case a.a h _ =>
+      exact h
+    exact beta_eq.symm h_beq₂
+  case right =>
+    apply beta_eq.trans
+    apply beta_eq.right
+    case a.a h _ =>
+      exact h
+    exact beta_eq.symm h_beq₂
+  case trans =>
+    apply beta_eq.trans
+    case a h _ _ _ =>
+      exact h
+    simp_all
+  case symm =>
+    apply beta_eq.symm
+    apply beta_eq.trans
+    exact h_beq₂
+    case a.a h _ =>
+      exact h
+
+end beta_eq
