SkLean/ToSk.lean
@@ -1,0 +1,123 @@
+import Mathlib.Tactic
+
+inductive LExpr where
+  | var   : ℕ     → LExpr
+  | app   : LExpr → LExpr → LExpr
+  | lam   : LExpr → LExpr
+  | m     : LExpr
+  | s     : LExpr
+  | k     : LExpr
+  | const : String → LExpr
+
+inductive SkExpr where
+  | s     : ℕ      → SkExpr
+  | k     : ℕ      → SkExpr
+  | m     : ℕ      → SkExpr
+  | call  : SkExpr → SkExpr → SkExpr
+  | hole  : SkExpr
+  | const : String → SkExpr
+  | lam   : SkExpr → SkExpr
+  | var   : ℕ      → SkExpr
+deriving BEq, Nonempty
+
+declare_syntax_cat skmexpr
+syntax "K" term                : skmexpr
+syntax "S" term                : skmexpr
+syntax "M" term                : skmexpr
+syntax "(" skmexpr skmexpr ")" : skmexpr
+syntax "?"                     : skmexpr
+syntax ident                   : skmexpr
+syntax "#" term                : skmexpr
+syntax "λ" skmexpr             : skmexpr
+syntax "(" skmexpr ")"         : skmexpr
+
+syntax " ⟪ " skmexpr " ⟫ "     : term
+syntax "SKM[ " skmexpr " ] "   : term
+
+macro_rules
+  | `(SKM[ $e:skmexpr ]) => `(⟪ $e ⟫)
+
+macro_rules
+  | `(⟪ K $e:term ⟫)                 => `(SkExpr.k $e)
+  | `(⟪ S $e:term ⟫)                 => `(SkExpr.s $e)
+  | `(⟪ M $e:term ⟫)                 => `(SkExpr.m $e)
+  | `(⟪ ? ⟫)                         => `(SkExpr.hole)
+  | `(⟪ $e:ident ⟫)                  => `($e)
+  | `(⟪ # $e:term ⟫)                 => `($e)
+  | `(⟪ ($e:skmexpr) ⟫)              => `(⟪$e⟫)
+  | `(⟪ λ $e:skmexpr ⟫)              => `(SkExpr.lam ⟪$e⟫)
+  | `(⟪ ($e₁:skmexpr $e₂:skmexpr) ⟫) => `(SkExpr.call ⟪ $e₁ ⟫ ⟪ $e₂ ⟫)
+
+namespace SkExpr
+
+def toStringImpl : SkExpr → String
+    | .s n          => s!"S {n}"
+    | .k n          => s!"K {n}"
+    | .m n          => s!"M {n}"
+    | .call lhs rhs => s!"({lhs.toStringImpl} {rhs.toStringImpl})"
+    | .const str    => s!"{str}"
+    | .hole         => "_"
+    | .lam body     => s!"λ {body.toStringImpl}"
+    | .var v        => s!"var {v}"
+
+instance : ToString SkExpr where
+  toString := SkExpr.toStringImpl
+
+def sum_universes : SkExpr → ℕ
+  | SKM[(K n)]       => n
+  | SKM[(S n)]       => n
+  | SKM[(M n)]       => n
+  | SKM[?]           => 0
+  | SKM[(lhs rhs)]   => lhs.sum_universes + rhs.sum_universes
+  | SKM[λ body]      => body.sum_universes
+  | x => 0
+
+def fill_universes : SkExpr → SkExpr
+  | SKM[((K _n) rhs)] => SKM[((K rhs.sum_universes) rhs)]
+  | SKM[((S _n) rhs)] => SKM[((S rhs.sum_universes) rhs)]
+  | SKM[((M _n) rhs)] => SKM[((M rhs.sum_universes) rhs)]
+  | x => x
+
+partial def eval_n (n : ℕ) (e : SkExpr) : SkExpr :=
+  if n = 0 then
+    e
+  else
+    let e' := match e with
+      | SKM[(((((K _n) _α) _β) x) _y)] => x
+      | SKM[(((((((S _n) _α) _β) _γ) x) y) z)] => eval_n n.pred SKM[((x z) (y z))]
+      | SKM[(lhs rhs)] => eval_n n.pred.pred SKM[((#(eval_n n.pred lhs)) (#(eval_n n.pred rhs)))] 
+      | x => x
+
+      eval_n  n.pred.pred.pred e'
+
+end SkExpr
+
+partial def normalize' (e : SkExpr) : SkExpr :=
+  match e with
+    | .lam (.var 0) => SKM[((((((S 0) ?) ?) ?) (((K 0) ?) ?)) (((K 0) ?) ?))]
+    | .k n => SKM[(K n)]
+    | .m n => SKM[(M n)]
+    | .s n => SKM[(S n)]
+    | .lam (.call lhs rhs) => normalize' SKM[((((((S 0) ?) ?) ?) #(normalize' (.lam lhs))) #(normalize' (.lam rhs)))]
+    | .lam x => SKM[((((K 0) ?) ?) #(normalize' x))]
+    | .const c => .const c
+    | .call lhs rhs => SKM[(#(normalize' lhs) #(normalize' rhs))]
+    | .var (v + 1) => normalize' $ .var v
+    | .var 0       => .var 0
+    | .hole => .hole
+
+partial def to_sk (e : LExpr) : SkExpr :=
+  match e with
+    | .lam (.var 0) => SKM[((((((S 0) ?) ?) ?) (((K 0) ?) ?)) (((K 0) ?) ?))]
+    | .k => SKM[K 0]
+    | .m => SKM[M 0]
+    | .s => SKM[S 0]
+    | (.app lhs rhs) => normalize' SKM[((#(to_sk lhs)) #(to_sk rhs))]
+    | .lam (.app lhs rhs) => normalize' SKM[(((((((S 0) ?) ?) ?) #(.lam $ to_sk lhs))) #(.lam $ to_sk rhs))]
+    | .lam x => SKM[((((K 0) ?) ?) #(to_sk x))]
+    | .const c => .const c
+    | .var (v + 1) => normalize' $ .var v
+    | .var 0       => .var 0
+
+#eval (.app (.app (LExpr.app (.app (.lam (.lam (.app (.app (.app .k (.app .m (.var 1))) (.var 0)) (.var 1)))) (.const "α")) (.const "β")) (.const "x")) (.const "y"))
+  |> (SkExpr.eval_n 10) ∘ to_sk
