SkLean/Typing2.lean
@@ -2,126 +2,31 @@ import SkLean.Ast2
 
 namespace valid_judgment
 
-lemma imp_exists_eval : valid_judgment e t → ∃ e', is_eval_once (trivial_typing e) e' := by
-  intro h_t
-  induction e
-  case m n =>
-    use SKM[(M n.succ)]
-    apply is_eval_once.m_m
-  case k n =>
-    use SKM[(K n.succ)]
-    apply is_eval_once.m_k
-  case s n =>
-    use SKM[(S n.succ)]
-    apply is_eval_once.m_s
-  case call lhs rhs ih₁ ih₂ =>
-    use SKM[(#(trivial_typing lhs) #(trivial_typing rhs))]
-    apply is_eval_once.m_call
-
-lemma call_exists_lhs_rhs_t : valid_judgment SKM[(lhs rhs)] t → ∃ t_lhs t_rhs, valid_judgment lhs t_lhs ∧ valid_judgment rhs t_rhs := by
-  intro h_t
-  cases h_t
-  case call_k x t_x t_y n h_t_x h_t_y =>
-    use (trivial_typing SKM[((K n) x)])
-    use t_y
-    exact ⟨valid_judgment.call_k₁ h_t_x, h_t_y⟩
-  case call_k₁ t_x n h_t_x =>
-    use (trivial_typing SKM[(K n)])
-    use t_x
-    exact ⟨by apply valid_judgment.k, h_t_x⟩
-  case call_s₁ t_x n h_t_x =>
-    use (trivial_typing SKM[(S n)])
-    use t_x
-    exact ⟨by apply valid_judgment.s, h_t_x⟩
-  case call_s₂ x t_x t_y n h_t_x h_t_y =>
-    use (trivial_typing SKM[((S n) x)])
-    use t_y
-    exact ⟨valid_judgment.call_s₁ h_t_x, h_t_y⟩
-  case call_s x y z t_x t_y t_call n h_t_x h_t_y h_t_z h_t_call h_u =>
-    use trivial_typing SKM[(((S n) x) y)]
-    simp_all
-    constructor
-    apply valid_judgment.call_s₂
-    exact h_t_x
-    exact h_t_y
-    use t_call
-  case call_m t n h_t =>
-    use (trivial_typing SKM[(M n)])
-    use t
-    exact ⟨valid_judgment.m n, h_t⟩
-  case call t_lhs t_rhs e' h_t_lhs h_t_rhs h_eval h_u =>
-    use t_lhs
-    use t_rhs
-
 lemma imp_m : valid_judgment e t → _root_.beta_eq (trivial_typing e) t := by
   intro h_t
   induction h_t
   repeat exact beta_eq.rfl
 
-theorem preservation_easy : valid_judgment e t → is_eval_once e e' → ∃ t', valid_judgment e' t' := by
-  intro h_t h_eval
-  induction h_t
-  case k n =>
-    use trivial_typing SKM[K n]
-    cases h_eval
-  case s n =>
-    use trivial_typing SKM[S n]
-    cases h_eval
-  case m n =>
-    use trivial_typing SKM[M n]
-    cases h_eval
-  case call_k₁ x t_x n h_t_x ih =>
-    cases h_eval
-    case left h =>
-      cases h
-  case call_s₁ x t_x n h_t_x ih =>
-    cases h_eval
-    case left h =>
-      cases h
-  case call_s₂ x t_x y t_y n h_t_x h_t_y ih₁ ih₂ =>
-    cases h_eval
-    case left h =>
-      cases h
-      case left h =>
+lemma k_preserved : valid_judgment SKM[((((K α) β) x) y)] t → beta_eq t α := by
+  intro h_t
+  cases h_t
+  case call t_rhs t_hs anything h_t_lhs h_t_y h_beq =>
+    cases h_t_lhs
+    case call h_t h_beq =>
+      cases h_t
+      case k h =>
         cases h
-  case call_k x t_x y t_y n h_t_x h_t_y ih₁ ih₂ =>
-    cases h_eval
-    use t_x
-    case left h =>
-      cases h
-      case left h =>
-        cases h
-  case call_s x z y t_call t_x t_y t_z n h_t_call h_t_x h_t_y h_t_z h_u ih₁ ih₂ ih₃ ih₄ =>
-    cases h_eval
-    use t_call
-    case left h =>
-      cases h
-      case left h =>
-        cases h
-        case left h =>
+        case call h _ _ =>
           cases h
-  case call_m e t n h_t h_eval₂ =>
-    cases h_eval
-    case m_k n =>
-      use trivial_typing SKM[(K n.succ)]
-      apply valid_judgment.k
-    case m_s n =>
-      use trivial_typing SKM[(S n.succ)]
-      apply valid_judgment.s
-    case m_m n =>
-      use trivial_typing SKM[(M n.succ)]
-      apply valid_judgment.m
-    case m_call t' lhs rhs =>
-      use trivial_typing SKM[(#(trivial_typing lhs) #(trivial_typing rhs))]
-      have ⟨t_lhs, t_rhs, h_t_lhs, h_t_rhs⟩ := h_t.call_exists_lhs_rhs_t
-      apply valid_judgment.call
-      apply valid_judgment.call_m
-      exact h_t_lhs
-      apply valid_judgment.call_m
-      exact h_t_rhs
-      apply is_eval_once.left
+          
+
+lemma well_typed_after_eval : is_eval_once e e' → valid_judgment e t → ∃ t', valid_judgment e' t' := by
+  intro h_eval h_t
+  match h : e with
+    | SKM[((((K α) β) x) y)] =>
       
       sorry
-    sorry
+    | SKM[((((((S α) β) γ) x) y) z)] => sorry
+    | SKM[(M (lhs rhs))] => sorry
 
 end valid_judgment
